<?xml version="1.0"?>
<rdf:RDF xmlns="http://www.semanticweb.org/ontologies/2024/asterisksinsports/"
     xml:base="http://www.semanticweb.org/ontologies/2024/asterisksinsports/"
     xmlns:dct="http://purl.org/dc/terms/"
     xmlns:owl="http://www.w3.org/2002/07/owl#"
     xmlns:rdf="http://www.w3.org/1999/02/22-rdf-syntax-ns#"
     xmlns:xml="http://www.w3.org/XML/1998/namespace"
     xmlns:xsd="http://www.w3.org/2001/XMLSchema#"
     xmlns:rdfs="http://www.w3.org/2000/01/rdf-schema#"
     xmlns:time="https://www.w3.org/2006/time#"
     xmlns:sports="https://sportschema.org/ontologies/main/"
     xmlns:perspectivisation="http://www.ontologydesignpatterns.org/ont/persp/perspectivisation.owl#">
    <owl:Ontology rdf:about="http://www.semanticweb.org/ontologies/2024/asterisksinsports"/>
    


    <!-- 
    ///////////////////////////////////////////////////////////////////////////////////////
    //
    // Object Properties
    //
    ///////////////////////////////////////////////////////////////////////////////////////
     -->

    


    <!-- http://www.semanticweb.org/ontologies/2024/asterisksinsports#achievedInSport -->

    <owl:ObjectProperty rdf:about="http://www.semanticweb.org/ontologies/2024/asterisksinsports#achievedInSport">
        <rdfs:domain rdf:resource="http://www.semanticweb.org/ontologies/2024/asterisksinsports#Achievement"/>
        <rdfs:range rdf:resource="http://www.semanticweb.org/ontologies/2024/asterisksinsports#Sport"/>
    </owl:ObjectProperty>
    


    <!-- http://www.semanticweb.org/ontologies/2024/asterisksinsports#characterisedBy -->

    <owl:ObjectProperty rdf:about="http://www.semanticweb.org/ontologies/2024/asterisksinsports#characterisedBy">
        <rdfs:domain rdf:resource="http://www.semanticweb.org/ontologies/2024/asterisksinsports#Viewpoint"/>
        <rdfs:range rdf:resource="http://www.semanticweb.org/ontologies/2024/asterisksinsports#AttitudeShift"/>
    </owl:ObjectProperty>
    


    <!-- http://www.semanticweb.org/ontologies/2024/asterisksinsports#comesFrom -->

    <owl:ObjectProperty rdf:about="http://www.semanticweb.org/ontologies/2024/asterisksinsports#comesFrom">
        <rdfs:domain rdf:resource="http://www.semanticweb.org/ontologies/2024/asterisksinsports#Actors"/>
        <rdfs:range rdf:resource="http://www.semanticweb.org/ontologies/2024/asterisksinsports#Provenance"/>
    </owl:ObjectProperty>
    


    <!-- http://www.semanticweb.org/ontologies/2024/asterisksinsports#createdBy -->

    <owl:ObjectProperty rdf:about="http://www.semanticweb.org/ontologies/2024/asterisksinsports#createdBy">
        <rdfs:domain rdf:resource="http://www.semanticweb.org/ontologies/2024/asterisksinsports#ControversyType"/>
        <rdfs:range rdf:resource="http://www.semanticweb.org/ontologies/2024/asterisksinsports#ElementOfControversy"/>
    </owl:ObjectProperty>
    


    <!-- http://www.semanticweb.org/ontologies/2024/asterisksinsports#determines -->

    <owl:ObjectProperty rdf:about="http://www.semanticweb.org/ontologies/2024/asterisksinsports#determines">
        <rdfs:domain rdf:resource="http://www.semanticweb.org/ontologies/2024/asterisksinsports#Viewpoint"/>
        <rdfs:range rdf:resource="http://www.semanticweb.org/ontologies/2024/asterisksinsports#PrimaryAttitude"/>
        <rdfs:range rdf:resource="http://www.semanticweb.org/ontologies/2024/asterisksinsports#Public_opinion"/>
        <rdfs:range rdf:resource="http://www.semanticweb.org/ontologies/2024/asterisksinsports#SecondaryAttitude"/>
    </owl:ObjectProperty>
    


    <!-- http://www.semanticweb.org/ontologies/2024/asterisksinsports#during -->

    <owl:ObjectProperty rdf:about="http://www.semanticweb.org/ontologies/2024/asterisksinsports#during">
        <rdfs:domain rdf:resource="http://www.semanticweb.org/ontologies/2024/asterisksinsports#Achievement"/>
        <rdfs:range rdf:resource="http://www.semanticweb.org/ontologies/2024/asterisksinsports#TimePeriod"/>
    </owl:ObjectProperty>
    


    <!-- http://www.semanticweb.org/ontologies/2024/asterisksinsports#hadParticipant -->

    <owl:ObjectProperty rdf:about="http://www.semanticweb.org/ontologies/2024/asterisksinsports#hadParticipant">
        <owl:inverseOf rdf:resource="http://www.semanticweb.org/ontologies/2024/asterisksinsports#participatedIn"/>
        <rdfs:domain rdf:resource="http://www.semanticweb.org/ontologies/2024/asterisksinsports#Achievement"/>
        <rdfs:range rdf:resource="http://www.semanticweb.org/ontologies/2024/asterisksinsports#Participant"/>
    </owl:ObjectProperty>
    


    <!-- http://www.semanticweb.org/ontologies/2024/asterisksinsports#hasAttitude -->

    <owl:ObjectProperty rdf:about="http://www.semanticweb.org/ontologies/2024/asterisksinsports#hasAttitude">
        <rdfs:domain rdf:resource="http://www.semanticweb.org/ontologies/2024/asterisksinsports#Actors"/>
        <rdfs:range rdf:resource="http://www.semanticweb.org/ontologies/2024/asterisksinsports#PrimaryAttitude"/>
        <rdfs:range rdf:resource="http://www.semanticweb.org/ontologies/2024/asterisksinsports#Public_opinion"/>
        <rdfs:range rdf:resource="http://www.semanticweb.org/ontologies/2024/asterisksinsports#SecondaryAttitude"/>
    </owl:ObjectProperty>
    


    <!-- http://www.semanticweb.org/ontologies/2024/asterisksinsports#hasViewpoint -->

    <owl:ObjectProperty rdf:about="http://www.semanticweb.org/ontologies/2024/asterisksinsports#hasViewpoint">
        <rdfs:domain rdf:resource="http://www.semanticweb.org/ontologies/2024/asterisksinsports#Actors"/>
        <rdfs:range rdf:resource="http://www.semanticweb.org/ontologies/2024/asterisksinsports#Viewpoint"/>
    </owl:ObjectProperty>
    


    <!-- http://www.semanticweb.org/ontologies/2024/asterisksinsports#influences -->

    <owl:ObjectProperty rdf:about="http://www.semanticweb.org/ontologies/2024/asterisksinsports#influences">
        <rdfs:domain rdf:resource="http://www.semanticweb.org/ontologies/2024/asterisksinsports#Context"/>
        <rdfs:range rdf:resource="http://www.semanticweb.org/ontologies/2024/asterisksinsports#PrimaryAttitude"/>
        <rdfs:range rdf:resource="http://www.semanticweb.org/ontologies/2024/asterisksinsports#Public_opinion"/>
        <rdfs:range rdf:resource="http://www.semanticweb.org/ontologies/2024/asterisksinsports#SecondaryAttitude"/>
    </owl:ObjectProperty>
    


    <!-- http://www.semanticweb.org/ontologies/2024/asterisksinsports#isInfluenced -->

    <owl:ObjectProperty rdf:about="http://www.semanticweb.org/ontologies/2024/asterisksinsports#isInfluenced">
        <rdfs:domain rdf:resource="http://www.semanticweb.org/ontologies/2024/asterisksinsports#Viewpoint"/>
        <rdfs:range rdf:resource="http://www.semanticweb.org/ontologies/2024/asterisksinsports#Context"/>
    </owl:ObjectProperty>
    


    <!-- http://www.semanticweb.org/ontologies/2024/asterisksinsports#locatedIn -->

    <owl:ObjectProperty rdf:about="http://www.semanticweb.org/ontologies/2024/asterisksinsports#locatedIn">
        <rdfs:domain rdf:resource="http://www.semanticweb.org/ontologies/2024/asterisksinsports#Achievement"/>
        <rdfs:range rdf:resource="http://www.semanticweb.org/ontologies/2024/asterisksinsports#Location"/>
    </owl:ObjectProperty>
    


    <!-- http://www.semanticweb.org/ontologies/2024/asterisksinsports#miredIn -->

    <owl:ObjectProperty rdf:about="http://www.semanticweb.org/ontologies/2024/asterisksinsports#miredIn">
        <rdfs:domain rdf:resource="http://www.semanticweb.org/ontologies/2024/asterisksinsports#Achievement"/>
        <rdfs:range rdf:resource="http://www.semanticweb.org/ontologies/2024/asterisksinsports#ControversyType"/>
    </owl:ObjectProperty>
    


    <!-- http://www.semanticweb.org/ontologies/2024/asterisksinsports#organisedBy -->

    <owl:ObjectProperty rdf:about="http://www.semanticweb.org/ontologies/2024/asterisksinsports#organisedBy">
        <rdfs:domain rdf:resource="http://www.semanticweb.org/ontologies/2024/asterisksinsports#Sport"/>
        <rdfs:range rdf:resource="http://www.semanticweb.org/ontologies/2024/asterisksinsports#GoverningBody"/>
    </owl:ObjectProperty>
    


    <!-- http://www.semanticweb.org/ontologies/2024/asterisksinsports#participatedIn -->

    <owl:ObjectProperty rdf:about="http://www.semanticweb.org/ontologies/2024/asterisksinsports#participatedIn">
        <rdfs:domain rdf:resource="http://www.semanticweb.org/ontologies/2024/asterisksinsports#Participant"/>
        <rdfs:range rdf:resource="http://www.semanticweb.org/ontologies/2024/asterisksinsports#Achievement"/>
    </owl:ObjectProperty>
    


    <!-- http://www.semanticweb.org/ontologies/2024/asterisksinsports#playedInSport -->

    <owl:ObjectProperty rdf:about="http://www.semanticweb.org/ontologies/2024/asterisksinsports#playedInSport">
        <rdfs:domain rdf:resource="http://www.semanticweb.org/ontologies/2024/asterisksinsports#Participant"/>
        <rdfs:range rdf:resource="http://www.semanticweb.org/ontologies/2024/asterisksinsports#Sport"/>
    </owl:ObjectProperty>
    


    <!-- http://www.semanticweb.org/ontologies/2024/asterisksinsports#towards -->

    <owl:ObjectProperty rdf:about="http://www.semanticweb.org/ontologies/2024/asterisksinsports#towards">
        <rdfs:domain rdf:resource="http://www.semanticweb.org/ontologies/2024/asterisksinsports#Viewpoint"/>
        <rdfs:range rdf:resource="http://www.semanticweb.org/ontologies/2024/asterisksinsports#Achievement"/>
    </owl:ObjectProperty>
    


    <!-- http://www.semanticweb.org/ontologies/2024/asterisksinsports#underAuspicesOf -->

    <owl:ObjectProperty rdf:about="http://www.semanticweb.org/ontologies/2024/asterisksinsports#underAuspicesOf">
        <rdfs:domain rdf:resource="http://www.semanticweb.org/ontologies/2024/asterisksinsports#Achievement"/>
        <rdfs:range rdf:resource="http://www.semanticweb.org/ontologies/2024/asterisksinsports#GoverningBody"/>
    </owl:ObjectProperty>
    


    <!-- 
    ///////////////////////////////////////////////////////////////////////////////////////
    //
    // Data properties
    //
    ///////////////////////////////////////////////////////////////////////////////////////
     -->

    


    <!-- http://www.semanticweb.org/ontologies/2024/asterisksinsports#hasSemanticValue -->

    <owl:DatatypeProperty rdf:about="http://www.semanticweb.org/ontologies/2024/asterisksinsports#hasSemanticValue">
        <rdfs:domain rdf:resource="http://www.semanticweb.org/ontologies/2024/asterisksinsports#ControversyType"/>
        <rdfs:range rdf:resource="http://www.w3.org/2000/01/rdf-schema#Literal"/>
    </owl:DatatypeProperty>
    


    <!-- 
    ///////////////////////////////////////////////////////////////////////////////////////
    //
    // Classes
    //
    ///////////////////////////////////////////////////////////////////////////////////////
     -->

    


    <!-- http://purl.org/dc/terms/Location -->

    <owl:Class rdf:about="http://purl.org/dc/terms/Location">
        <owl:equivalentClass rdf:resource="http://www.semanticweb.org/ontologies/2024/asterisksinsports#Location"/>
    </owl:Class>
    


    <!-- http://www.ontologydesignpatterns.org/ont/persp/perspectivisation.owl#Attitude -->

    <owl:Class rdf:about="http://www.ontologydesignpatterns.org/ont/persp/perspectivisation.owl#Attitude">
        <rdfs:label>Attitude</rdfs:label>
        <rdfs:label>The behavior of an Actor towards the result of a competition.</rdfs:label>
    </owl:Class>
    


    <!-- http://www.ontologydesignpatterns.org/ont/persp/perspectivisation.owl#Background -->

    <owl:Class rdf:about="http://www.ontologydesignpatterns.org/ont/persp/perspectivisation.owl#Background">
        <rdfs:comment>The factors that inform the decision or opinion of an Actor. 

They can be cultural, technological, historical, social, political, or economic.</rdfs:comment>
        <rdfs:label>Background</rdfs:label>
    </owl:Class>
    


    <!-- http://www.ontologydesignpatterns.org/ont/persp/perspectivisation.owl#Cut -->

    <owl:Class rdf:about="http://www.ontologydesignpatterns.org/ont/persp/perspectivisation.owl#Cut">
        <rdfs:label>Cut</rdfs:label>
        <rdfs:label>Represents the moment where and the motivations for Actors change an Attitude.</rdfs:label>
    </owl:Class>
    


    <!-- http://www.ontologydesignpatterns.org/ont/persp/perspectivisation.owl#Eventuality -->

    <owl:Class rdf:about="http://www.ontologydesignpatterns.org/ont/persp/perspectivisation.owl#Eventuality"/>
    


    <!-- http://www.ontologydesignpatterns.org/ont/persp/perspectivisation.owl#Lens -->

    <owl:Class rdf:about="http://www.ontologydesignpatterns.org/ont/persp/perspectivisation.owl#Lens">
        <rdfs:comment>Represent all the factors that inform the decision or opinion making of an Actor.</rdfs:comment>
        <rdfs:label>Lens</rdfs:label>
    </owl:Class>
    


    <!-- http://www.semanticweb.org/ontologies/2024/asterisksinsports#Achievement -->

    <owl:Class rdf:about="http://www.semanticweb.org/ontologies/2024/asterisksinsports#Achievement">
        <rdfs:subClassOf rdf:resource="http://www.ontologydesignpatterns.org/ont/persp/perspectivisation.owl#Eventuality"/>
        <rdfs:comment>Represents a sporting accomplishment made by a sportsperson or a group of sportspeople. This ranges from winning championship titles, through outstanding performances and breaking records to just qualifying to participate at a certain event.</rdfs:comment>
        <rdfs:label>Achievement</rdfs:label>
    </owl:Class>
    


    <!-- http://www.semanticweb.org/ontologies/2024/asterisksinsports#Actors -->

    <owl:Class rdf:about="http://www.semanticweb.org/ontologies/2024/asterisksinsports#Actors">
        <rdfs:comment>Representation of both participants and non-participants in a sporting event.</rdfs:comment>
        <rdfs:label>Actors</rdfs:label>
    </owl:Class>
    


    <!-- http://www.semanticweb.org/ontologies/2024/asterisksinsports#AttitudeShift -->

    <owl:Class rdf:about="http://www.semanticweb.org/ontologies/2024/asterisksinsports#AttitudeShift">
        <rdfs:subClassOf rdf:resource="http://www.ontologydesignpatterns.org/ont/persp/perspectivisation.owl#Cut"/>
        <rdfs:comment>Represents a personal shift of attitute regarding a sporting achievement.</rdfs:comment>
        <rdfs:label>Attitude shift</rdfs:label>
    </owl:Class>
    


    <!-- http://www.semanticweb.org/ontologies/2024/asterisksinsports#Context -->

    <owl:Class rdf:about="http://www.semanticweb.org/ontologies/2024/asterisksinsports#Context">
        <rdfs:subClassOf rdf:resource="http://www.ontologydesignpatterns.org/ont/persp/perspectivisation.owl#Background"/>
        <rdfs:comment>Represents context and a plethora of external factors (e.g. media coverage, personal knowledge, cultural and moral values) influencing outlooks on a sporting achievement.</rdfs:comment>
        <rdfs:label>Context</rdfs:label>
    </owl:Class>
    


    <!-- http://www.semanticweb.org/ontologies/2024/asterisksinsports#ContextualFactors -->

    <owl:Class rdf:about="http://www.semanticweb.org/ontologies/2024/asterisksinsports#ContextualFactors">
        <rdfs:subClassOf rdf:resource="http://www.semanticweb.org/ontologies/2024/asterisksinsports#ControversyType"/>
        <rdfs:comment>Represents the cases, where the legitimacy of an achievement has been challenged due to factors outside of the actual sporting results.</rdfs:comment>
        <rdfs:label>Contextual factors</rdfs:label>
    </owl:Class>
    


    <!-- http://www.semanticweb.org/ontologies/2024/asterisksinsports#ControversyType -->

    <owl:Class rdf:about="http://www.semanticweb.org/ontologies/2024/asterisksinsports#ControversyType">
        <rdfs:comment>Represents the type of controversy surrounding a sporting achievement.</rdfs:comment>
        <rdfs:label>Controversy type</rdfs:label>
    </owl:Class>
    


    <!-- http://www.semanticweb.org/ontologies/2024/asterisksinsports#Doping -->

    <owl:Class rdf:about="http://www.semanticweb.org/ontologies/2024/asterisksinsports#Doping">
        <rdfs:subClassOf rdf:resource="http://www.semanticweb.org/ontologies/2024/asterisksinsports#ControversyType"/>
        <rdfs:comment>Represents cases, where a sporting achievement has been surrounded by controversiues due to improving performance through illicit chemicals.</rdfs:comment>
        <rdfs:label>Doping</rdfs:label>
    </owl:Class>
    


    <!-- http://www.semanticweb.org/ontologies/2024/asterisksinsports#ElementOfControversy -->

    <owl:Class rdf:about="http://www.semanticweb.org/ontologies/2024/asterisksinsports#ElementOfControversy">
        <rdfs:comment>Represents an element that has lead to existence of, or the root cause of a controversy regarding an Achievement.</rdfs:comment>
        <rdfs:label>Element of controversy</rdfs:label>
    </owl:Class>
    


    <!-- http://www.semanticweb.org/ontologies/2024/asterisksinsports#Ethics -->

    <owl:Class rdf:about="http://www.semanticweb.org/ontologies/2024/asterisksinsports#Ethics">
        <rdfs:subClassOf rdf:resource="http://www.semanticweb.org/ontologies/2024/asterisksinsports#ControversyType"/>
        <rdfs:comment>Represents cases, where a sporting achievement has been surrounded by controversies due to ethical considerations.</rdfs:comment>
        <rdfs:label>Ethics</rdfs:label>
    </owl:Class>
    


    <!-- http://www.semanticweb.org/ontologies/2024/asterisksinsports#Gender -->

    <owl:Class rdf:about="http://www.semanticweb.org/ontologies/2024/asterisksinsports#Gender">
        <rdfs:subClassOf rdf:resource="http://www.semanticweb.org/ontologies/2024/asterisksinsports#ControversyType"/>
        <rdfs:comment>Represents cases, where a sporting achievement has been surrounded by controversies due to athletes gender/hormone levels.</rdfs:comment>
        <rdfs:label>Gender issues</rdfs:label>
    </owl:Class>
    


    <!-- http://www.semanticweb.org/ontologies/2024/asterisksinsports#GoverningBody -->

    <owl:Class rdf:about="http://www.semanticweb.org/ontologies/2024/asterisksinsports#GoverningBody">
        <owl:equivalentClass rdf:resource="https://sportschema.org/ontologies/main/GoverningBody"/>
        <rdfs:subClassOf rdf:resource="http://www.semanticweb.org/ontologies/2024/asterisksinsports#NonParticipant"/>
        <rdfs:comment>Represents the governing body, under whose auspices the event was run, in which an achievement has been made in.</rdfs:comment>
        <rdfs:label>Governing body</rdfs:label>
    </owl:Class>
    


    <!-- http://www.semanticweb.org/ontologies/2024/asterisksinsports#Location -->

    <owl:Class rdf:about="http://www.semanticweb.org/ontologies/2024/asterisksinsports#Location">
        <rdfs:comment>Represents the singular physical location (if possible), or a broader geographical context, where an Achievement has taken place.</rdfs:comment>
        <rdfs:label>Location</rdfs:label>
    </owl:Class>
    


    <!-- http://www.semanticweb.org/ontologies/2024/asterisksinsports#NonParticipant -->

    <owl:Class rdf:about="http://www.semanticweb.org/ontologies/2024/asterisksinsports#NonParticipant">
        <rdfs:subClassOf rdf:resource="http://www.semanticweb.org/ontologies/2024/asterisksinsports#Actors"/>
        <owl:disjointWith rdf:resource="http://www.semanticweb.org/ontologies/2024/asterisksinsports#Participant"/>
        <rdfs:comment>It represents people who do not participate directly in sporting events, such as fans, national governments, and the press.</rdfs:comment>
        <rdfs:label>Non-participant</rdfs:label>
    </owl:Class>
    


    <!-- http://www.semanticweb.org/ontologies/2024/asterisksinsports#Officiating -->

    <owl:Class rdf:about="http://www.semanticweb.org/ontologies/2024/asterisksinsports#Officiating">
        <rdfs:subClassOf rdf:resource="http://www.semanticweb.org/ontologies/2024/asterisksinsports#ControversyType"/>
        <rdfs:comment>Represents cases, where a sporting achievement has been surrounded by controversies due to officiating mistakes and/or corrupt officials.</rdfs:comment>
        <rdfs:label>Officiating</rdfs:label>
    </owl:Class>
    


    <!-- http://www.semanticweb.org/ontologies/2024/asterisksinsports#Participant -->

    <owl:Class rdf:about="http://www.semanticweb.org/ontologies/2024/asterisksinsports#Participant">
        <owl:equivalentClass rdf:resource="https://sportschema.org/ontologies/main/Agent"/>
        <rdfs:subClassOf rdf:resource="http://www.semanticweb.org/ontologies/2024/asterisksinsports#Actors"/>
        <rdfs:comment>Representation of a specific sportsperson, or a group of sportspeople participating in a club or representing their nation in a sporting competition.</rdfs:comment>
        <rdfs:label>Participant</rdfs:label>
    </owl:Class>
    


    <!-- http://www.semanticweb.org/ontologies/2024/asterisksinsports#PrimaryAttitude -->

    <owl:Class rdf:about="http://www.semanticweb.org/ontologies/2024/asterisksinsports#PrimaryAttitude">
        <rdfs:subClassOf rdf:resource="http://www.ontologydesignpatterns.org/ont/persp/perspectivisation.owl#Attitude"/>
        <owl:disjointWith rdf:resource="http://www.semanticweb.org/ontologies/2024/asterisksinsports#SecondaryAttitude"/>
        <rdfs:comment>The primary decision of an Actor, in regards to some Achievement.</rdfs:comment>
        <rdfs:label>Primary decision</rdfs:label>
    </owl:Class>
    


    <!-- http://www.semanticweb.org/ontologies/2024/asterisksinsports#Provenance -->

    <owl:Class rdf:about="http://www.semanticweb.org/ontologies/2024/asterisksinsports#Provenance">
        <rdfs:comment>Represents the place, from which a person comes from, either a participant, or a non-participant.</rdfs:comment>
        <rdfs:label>Provenance</rdfs:label>
    </owl:Class>
    


    <!-- http://www.semanticweb.org/ontologies/2024/asterisksinsports#Public_opinion -->

    <owl:Class rdf:about="http://www.semanticweb.org/ontologies/2024/asterisksinsports#Public_opinion">
        <rdfs:subClassOf rdf:resource="http://www.ontologydesignpatterns.org/ont/persp/perspectivisation.owl#Attitude"/>
        <rdfs:comment>Manifestation of an Actor about the results of a Achievement.</rdfs:comment>
        <rdfs:label>Public opinion</rdfs:label>
    </owl:Class>
    


    <!-- http://www.semanticweb.org/ontologies/2024/asterisksinsports#RuleViolation -->

    <owl:Class rdf:about="http://www.semanticweb.org/ontologies/2024/asterisksinsports#RuleViolation">
        <rdfs:subClassOf rdf:resource="http://www.semanticweb.org/ontologies/2024/asterisksinsports#ControversyType"/>
        <rdfs:comment>Represents cases, where a sporting achievement has been surrounded by controversies due to violating the ruleset of the sport or competition.</rdfs:comment>
        <rdfs:label>Rule violation</rdfs:label>
    </owl:Class>
    


    <!-- http://www.semanticweb.org/ontologies/2024/asterisksinsports#SecondaryAttitude -->

    <owl:Class rdf:about="http://www.semanticweb.org/ontologies/2024/asterisksinsports#SecondaryAttitude">
        <rdfs:subClassOf rdf:resource="http://www.ontologydesignpatterns.org/ont/persp/perspectivisation.owl#Attitude"/>
        <rdfs:comment>The secondary decision of an Actor, towards a certain Achievement, coming due to a change of viewpoint.</rdfs:comment>
        <rdfs:label>Secondary decision</rdfs:label>
    </owl:Class>
    


    <!-- http://www.semanticweb.org/ontologies/2024/asterisksinsports#Sport -->

    <owl:Class rdf:about="http://www.semanticweb.org/ontologies/2024/asterisksinsports#Sport">
        <rdfs:comment>Represents the sport, in which an Achievement has been made in.</rdfs:comment>
        <rdfs:label>Sport</rdfs:label>
    </owl:Class>
    


    <!-- http://www.semanticweb.org/ontologies/2024/asterisksinsports#Technology -->

    <owl:Class rdf:about="http://www.semanticweb.org/ontologies/2024/asterisksinsports#Technology">
        <rdfs:subClassOf rdf:resource="http://www.semanticweb.org/ontologies/2024/asterisksinsports#ControversyType"/>
        <rdfs:comment>Represents cases, where a sporting achievement has been surrounded by controversies due to technological advancements impacting the result.</rdfs:comment>
        <rdfs:label>Technological advancements</rdfs:label>
    </owl:Class>
    


    <!-- http://www.semanticweb.org/ontologies/2024/asterisksinsports#TimePeriod -->

    <owl:Class rdf:about="http://www.semanticweb.org/ontologies/2024/asterisksinsports#TimePeriod">
        <owl:equivalentClass rdf:resource="https://www.w3.org/2006/time#TemporalEntity"/>
        <rdfs:comment>Represents the timeframe, when an Achievement has taken place.</rdfs:comment>
        <rdfs:label>Time period</rdfs:label>
    </owl:Class>
    


    <!-- http://www.semanticweb.org/ontologies/2024/asterisksinsports#Viewpoint -->

    <owl:Class rdf:about="http://www.semanticweb.org/ontologies/2024/asterisksinsports#Viewpoint">
        <rdfs:subClassOf rdf:resource="http://www.ontologydesignpatterns.org/ont/persp/perspectivisation.owl#Lens"/>
        <rdfs:comment>Represents a perspective of an individual towards a sporting achievement.</rdfs:comment>
        <rdfs:label>Viewpoint</rdfs:label>
    </owl:Class>
    


    <!-- https://sportschema.org/ontologies/main/Agent -->

    <owl:Class rdf:about="https://sportschema.org/ontologies/main/Agent">
        <rdfs:comment>The person or institution that competes on a competition.</rdfs:comment>
        <rdfs:label>Agent</rdfs:label>
    </owl:Class>
    


    <!-- https://sportschema.org/ontologies/main/GoverningBody -->

    <owl:Class rdf:about="https://sportschema.org/ontologies/main/GoverningBody"/>
    


    <!-- https://www.w3.org/2006/time#TemporalEntity -->

    <owl:Class rdf:about="https://www.w3.org/2006/time#TemporalEntity">
        <rdfs:label>TemporalEntity</rdfs:label>
    </owl:Class>
    


    <!-- 
    ///////////////////////////////////////////////////////////////////////////////////////
    //
    // General axioms
    //
    ///////////////////////////////////////////////////////////////////////////////////////
     -->

    <rdf:Description>
        <rdf:type rdf:resource="http://www.w3.org/2002/07/owl#AllDisjointClasses"/>
        <owl:members rdf:parseType="Collection">
            <rdf:Description rdf:about="http://www.semanticweb.org/ontologies/2024/asterisksinsports#ContextualFactors"/>
            <rdf:Description rdf:about="http://www.semanticweb.org/ontologies/2024/asterisksinsports#Doping"/>
            <rdf:Description rdf:about="http://www.semanticweb.org/ontologies/2024/asterisksinsports#Ethics"/>
            <rdf:Description rdf:about="http://www.semanticweb.org/ontologies/2024/asterisksinsports#Gender"/>
            <rdf:Description rdf:about="http://www.semanticweb.org/ontologies/2024/asterisksinsports#Officiating"/>
            <rdf:Description rdf:about="http://www.semanticweb.org/ontologies/2024/asterisksinsports#RuleViolation"/>
            <rdf:Description rdf:about="http://www.semanticweb.org/ontologies/2024/asterisksinsports#Technology"/>
        </owl:members>
    </rdf:Description>
</rdf:RDF>



<!-- Generated by the OWL API (version 4.5.29.2024-05-13T12:11:03Z) https://github.com/owlcs/owlapi -->

